# **Endogeneity in the CAPM**

This repository involves my own research on the problem of endogeneity in the Capital Asset Pricing Model (CAPM). I present the problem and the sources of endogeneity in CAPM, show how to approximate the resulting estimation bias and assess its impact in certain uses, such as VaR, and propose ways of adjusting the estimator to reduce the bias. Apart from the basic definitions, all the ideas, formulas, derivations and calculations are developed fully by me, unless specified otherwise.


## Introduction

CAPM is a broadly utilized model in the financial industry. Although it was primarily meant to describe the expected returns of portfolios in the equilibrium in relation to the expected excess return of the market portfolio, its usefulness in terms of describing the structure of relationship between different market factors is very often leveraged. 

$$E[r_i]=r_f+\beta_i(E[r_m]-r_f)$$

More specifically, an additional assumption of linear relationship between the returns is taken, so that a simple linear regression formula with a single explanatory variable is obtained. Additionally, the risk-free rate can be omitted in the equation, and in certain cases (such as risk modelling) the intercept can be assumed to be equal to zero. Note that, if daily returns are considered, their expected values will usually be very close to 0 (especially for the risk-free rate), which justifies such approach to the analysis. Such model is sometimes referred to as <b>Beta Model</b> (we will use this name from now on). The most common practice is to take some major index on a given market as a proxy for the market portfolio, and use its returns ($r_I$) as an explanatory variable, which is supposed to represent the systematic component of a given market factor. 

$$r_i = \alpha_i + \beta_i r_I + \varepsilon_i$$

However, one should note that indices, or any other proxies of market portfolios, are never equivalent to the systematic factors. Otherwise, the relationship described by the above formula would lead to contradictions:
- For the market factors (e.g., stocks) constituting the corresponding index, how is it possible that the moves of this index cause their moves if they have been used to construct it in the first place?
- Even if a given market factor does not constitute the index, how would this causal relationship work?

In reality, there is a latent (unobservable) variable representing the systemic factor, which impacts the moves of particular market factors. It can be thought of as the extent of market participants decisions which is due to their perspective on general conditions on a given market.


## True DGP in the Beta Model

We assume we have a homogenous cluster of $ğ‘$ market factors, which returns are dependent on a systematic component ($ğ‘ $) and an idiosyncratic component. There is a single systematic component for all market factors in the cluster, and there is a unique idiosyncratic component for each market factor. Idiosyncratic components of each two different market factors are independent. Thus, we have the following true Data Generating Process (DGP) in our Beta Model:

$$ğ‘Ÿ_ğ‘–=ğ›½_ğ‘– ğ‘Ÿ_ğ‘ +ğœ€_ğ‘–,$$

where:
- $ğ‘Ÿ_ğ‘–$ â€“ return of the market factor $ğ‘–$, $ğ‘–=1,â€¦,ğ‘$;
- $ğ›½_ğ‘–$ â€“ beta coefficient of market factor $ğ‘–$;
- $ğ‘Ÿ_ğ‘ $ â€“ return of the systematic component;
- $ğœ€_ğ‘–$ â€“ idiosyncratic component of the market factor $ğ‘–$ return.

Distinction into systematic component and idiosyncratic component is abstract. Return of the systemic component is unobservable (as is the idiosyncratic component). In reality we can only observe return of an index ($ğ¼$), which is supposed to reflect the impact of systematic component. We assume that return of the index is a weighted average of the returns of $ğ‘›$ market factors belonging to the cluster:

$$ğ‘Ÿ_ğ¼ = ğ‘Ÿ_1 ğ‘¤_1 + ğ‘Ÿ_2 ğ‘¤_2 + â€¦ + ğ‘Ÿ_ğ‘› ğ‘¤_ğ‘› = \sum_{ğ‘—=1}^{ğ‘›} \left(ğ›½_ğ‘— ğ‘Ÿ_ğ‘  + ğœ€_ğ‘— \right) ğ‘¤_ğ‘— = \sum_{ğ‘—=1}^{ğ‘›} \left(ğ›½_ğ‘—Ã—ğ‘Ÿ_ğ‘  \right) ğ‘¤_ğ‘— + \sum_{ğ‘—=1}^{ğ‘›} ğœ€_ğ‘—Ã—ğ‘¤_ğ‘—,$$

where:
- $ğ‘Ÿ_ğ¼$ â€“ return of the index $ğ¼$;
- $ğ‘¤_ğ‘—$ â€“ weight of the market factor $ğ‘—$, $ğ‘—=1,â€¦,ğ‘›â‰¤ğ‘$;
- $ğ‘¤_1+ğ‘¤_2+â€¦+ğ‘¤_ğ‘›=1$.

In general, the higher the $ğ‘›$ is (or, the lower the weights are), the better the index reflects the systematic component.


## **The phenomena of endogeneity and its implications**

An explanatory variable is said to be endogenous when it is correlated with error term, i.e., $ğ¸[ğœ€|ğ‘¥]â‰ 0$.

Consequences:

1. Bias of the least squares estimator:

$$ E\left[{\hat{ğ›½}}^{ğ‘‚ğ¿ğ‘†} \right] = ğ›½ + (ğ‘¿^{ğ‘‡} ğ‘¿)^{âˆ’1} ğ‘¿^{ğ‘‡} ğ¸[\varepsilon|ğ‘¿] $$

2. Inconsistency of the least squares estimator:

$$ p-\lim_{N \to {+\infty}} â¡{\hat{ğ›½}}^{ğ‘‚ğ¿ğ‘†} = \beta + p-\lim_{N \to {+\infty}}â¡ { \left( \frac{1}{N} ğ‘¿^{ğ‘‡} ğ‘¿ \right)^{âˆ’1} \frac{1}{N} ğ‘¿^{ğ‘‡} ğ¸[\varepsilon|ğ‘¿]} $$

Standard sources of endogeneity:

1) <b>Omitted variable bias</b>

2) <b>Measurement error</b>

3) Simultaneous causality


## **Sources of endogeneity in the Beta Model**

1. Omitted variable in the Beta model â€“ idiosyncratic component

$$ ğ‘ğ‘œğ‘£ \left(ğ‘Ÿ_ğ¼, ğœ€_{ğ‘˜â‰¤ğ‘›} \right) = ğ‘ğ‘œğ‘£ \left( \sum_{ğ‘—=1}^{ğ‘›} ğ‘¤_ğ‘— ğ›½_ğ‘— ğ‘Ÿ_ğ‘  + \sum_{ğ‘—=1}^{ğ‘›} ğœ€_ğ‘— ğ‘¤_ğ‘—, ğœ€_{ğ‘˜â‰¤ğ‘›} \right) = ğ¸ \left[ ğ‘¤_{ğ‘˜â‰¤ğ‘›} ğœ€_{ğ‘˜â‰¤ğ‘›}^{2} \right] â‰  0 $$

2. Measurement error â€“ index is not equivalent to the systemic component

$$ ğ‘Ÿ_ğ‘– = ğ›½_ğ‘– ğ‘Ÿ_ğ‘  + ğœ€_ğ‘– $$
$$ ğ‘Ÿ_ğ¼ = ğ‘Ÿ_ğ‘  \sum_{ğ‘—=1}^{ğ‘›} ğ›½_ğ‘— ğ‘¤_ğ‘— + \sum_{ğ‘—=1}^{ğ‘›} ğœ€_ğ‘— ğ‘¤_ğ‘— â‡’ ğ‘Ÿ_ğ‘  = \frac{ğ‘Ÿ_ğ¼}{\sum_{ğ‘—=1}^{ğ‘›} ğ›½_ğ‘— ğ‘¤_ğ‘—} âˆ’ \frac{\sum_{ğ‘—=1}^{ğ‘›} ğœ€_ğ‘— ğ‘¤_ğ‘—}{\sum_{ğ‘—=1}^{ğ‘›} ğ›½_ğ‘— ğ‘¤_ğ‘—} $$
$$ ğ‘Ÿ_ğ‘– = ğ›½_ğ‘– \left( \frac{ğ‘Ÿ_ğ¼}{\sum_{ğ‘—=1}^{ğ‘›} ğ›½_ğ‘— ğ‘¤_ğ‘—} âˆ’ \frac{\sum_{ğ‘—=1}^{ğ‘›} ğœ€_ğ‘— ğ‘¤_ğ‘—}{\sum_{ğ‘—=1}^{ğ‘›} ğ›½_ğ‘— ğ‘¤_ğ‘—} \right) + ğœ€_ğ‘– = \frac{ğ›½_ğ‘– ğ‘Ÿ_ğ¼}{\sum_{ğ‘—=1}^{ğ‘›} ğ›½_ğ‘— ğ‘¤_ğ‘—} + \left( âˆ’ \frac{ğ›½_ğ‘–}{\sum_{ğ‘—=1}^{ğ‘›} ğ›½_ğ‘— ğ‘¤_ğ‘—} \left( \sum_{ğ‘—=1}^{ğ‘›} ğœ€_ğ‘— ğ‘¤_ğ‘— \right) + ğœ€_ğ‘– \right) $$

Even if $ğ‘–>ğ‘›$, we have: 

$$ ğ‘ğ‘œğ‘£ \left( \sum_{ğ‘—=1}^{ğ‘›} ğ‘¤_ğ‘— ğ›½_ğ‘— ğ‘Ÿ_ğ‘  + \sum_{ğ‘—=1}^{ğ‘›} ğœ€_ğ‘— ğ‘¤_ğ‘— , \left( âˆ’ \frac{ğ›½_ğ‘–}{\sum_{ğ‘—=1}^{ğ‘›} ğ›½_ğ‘— ğ‘¤_ğ‘—} \left( \sum_{ğ‘—=1}^{ğ‘›} ğœ€_ğ‘— ğ‘¤_ğ‘— \right) + ğœ€_ğ‘– \right) \right) = - \frac{ğ›½_ğ‘–}{\sum_{ğ‘—=1}^{ğ‘›} ğ›½_ğ‘— ğ‘¤_ğ‘—} ğ¸ \left[ \left( \sum_{ğ‘—=1}^{ğ‘›} ğœ€_ğ‘— ğ‘¤_ğ‘— \right)^{2} \right] â‰  0 $$

The first issue concerns only index components, while the second concerns all market factors in a given cluster. 


## **Coefficients in a simple framework**

Consider the following framework. We have $ğ‘â‰¥2$ market factors in a cluster, $ğ‘›âˆˆ[2,ğ‘]$ of them compose an index. We assume all weights are equal, i.e., $ğ‘¤_ğ‘—=\frac{1}{ğ‘›}$ for $ğ‘—=1,â€¦,ğ‘›$, and all betas are equal, i.e., $ğ›½_ğ‘–=ğ›½$ for $ğ‘–=1,â€¦,ğ‘$. Additionally, we assume all market factorsâ€™ returns, as well as the systematic component return, follow a standard normal distribution, i.e., $ğ‘Ÿ_ğ‘  \sim ğ‘(0,1)$ and $ğ‘Ÿ_ğ‘– \sim ğ‘(0,1)$ for $ğ‘–=1,â€¦,ğ‘$. We want to calibrate coefficients of correlation with the systematic component for all market factors in a cluster over some time interval $ğ‘‡$. 

Variance of the idiosyncratic component:

$$ \forall_{ğ‘–=1,â€¦,ğ‘} ğœ_{ğ‘–}^{2} â‰¡ ğ‘£ğ‘ğ‘Ÿ(ğ‘Ÿ_ğ‘–) = ğ‘£ğ‘ğ‘Ÿ \left( ğ›½ ğ‘Ÿ_ğ‘  + ğœ€_ğ‘– \right) = 1 âŸ¹ ğ‘£ğ‘ğ‘Ÿ (ğœ€_ğ‘–) = 1âˆ’ğ›½^2 $$

Index return and its variance:

$$ ğ‘Ÿ_ğ¼ = \frac{(ğ›½ğ‘Ÿ_ğ‘ +ğœ€_1 ) + (ğ›½ğ‘Ÿ_ğ‘ +ğœ€_2) + â€¦ + (ğ›½ğ‘Ÿ_ğ‘ +ğœ€_ğ‘›)}{ğ‘›} = ğ›½ ğ‘Ÿ_ğ‘  + \frac{1}{ğ‘›} \sum_{ğ‘—=1}^{ğ‘›} ğœ€_ğ‘— $$

$$ ğœ_{ğ¼}^{2} â‰¡ ğ‘£ğ‘ğ‘Ÿ(ğ‘Ÿ_ğ¼ ) = ğ‘£ğ‘ğ‘Ÿ \left( ğ›½ ğ‘Ÿ_ğ‘  + \frac{1}{ğ‘›} \sum_{ğ‘—=1}^{ğ‘›} ğœ€_ğ‘— \right) = ğ›½^2 + \frac{1}{ğ‘›^2} \sum_{ğ‘—=1}^{ğ‘›} \left( 1âˆ’ğ›½^2 \right) = ğ›½^2 + \frac{1âˆ’ğ›½^2}{ğ‘›} $$

Covariance and correlation of a component market factor return:

$$ ğ‘ğ‘œğ‘£ \left( ğ‘Ÿ_ğ¼ , ğ‘Ÿ_{ğ‘˜â‰¤ğ‘›} \right) = ğ¸ \left[ \left( ğ›½ ğ‘Ÿ_ğ‘  + \frac{1}{ğ‘›} \sum_{ğ‘—=1}^{ğ‘›} ğœ€_ğ‘— \right) \left( ğ›½ ğ‘Ÿ_ğ‘  + ğœ€_{ğ‘˜â‰¤ğ‘›} \right) \right] = ğ¸ \left[ ğ›½^2 ğ‘Ÿ_{ğ‘ }^{2} + \frac{ğœ€_{ğ‘˜â‰¤ğ‘›}^{2}}{ğ‘›} \right] = ğ›½^2 + \frac{1âˆ’ğ›½^2}{ğ‘›} $$

$$ ğœŒ_{ğ‘Ÿ_ğ¼, ğ‘Ÿ_{ğ‘˜â‰¤ğ‘›}} = \frac{ğ›½^2 + \frac{1âˆ’ğ›½^2}{ğ‘›}}{\sqrt{ğ›½^2 + \frac{1âˆ’ğ›½^2}{ğ‘›}}} = \sqrt{\frac{(ğ‘›âˆ’1) ğ›½^2 + 1}{ğ‘›}} âŸ¹ ğ›½ = \sqrt{ \frac{ ğ‘› ğœŒ_{ğ‘Ÿ_ğ¼, ğ‘Ÿ_{ğ‘˜â‰¤ğ‘›}}^{2} âˆ’ 1}{ğ‘›âˆ’1} } $$

Note that, since the volatilities of all market factors and of the systematic component are equal to 1, betas are equal to correlations, and thus: 

$$ \rho_{ğ‘Ÿ_s, ğ‘Ÿ_{ğ‘˜â‰¤ğ‘›}} = \sqrt{ \frac{ ğ‘› ğœŒ_{ğ‘Ÿ_ğ¼, ğ‘Ÿ_{ğ‘˜â‰¤ğ‘›}}^{2} âˆ’ 1}{ğ‘›âˆ’1} } $$

Hence, we get the following unbiased estimator of the correlation with systematic component as a function of the obtained estimator of the correlation with its proxy (index):

$$ \hat{\rho_{ğ‘Ÿ_s, ğ‘Ÿ_{ğ‘˜â‰¤ğ‘›}}} = \sqrt{ \frac{ ğ‘› \hat{ğœŒ_{ğ‘Ÿ_ğ¼, ğ‘Ÿ_{ğ‘˜â‰¤ğ‘›}}}^{2} âˆ’ 1}{ğ‘›âˆ’1} } $$ 

Covariance and correlation of a non-component market factor return:

$$ ğ‘ğ‘œğ‘£ \left( ğ‘Ÿ_ğ¼ , ğ‘Ÿ_{ğ‘˜ \gt ğ‘›} \right) = ğ¸ \left[ \left( ğ›½ ğ‘Ÿ_ğ‘  + \frac{1}{ğ‘›} \sum_{ğ‘—=1}^{ğ‘›} ğœ€_ğ‘— \right) \left( ğ›½ ğ‘Ÿ_ğ‘  + ğœ€_{ğ‘˜ \gt ğ‘›} \right) \right] = ğ¸ \left[ ğ›½^2 ğ‘Ÿ_{ğ‘ }^{2} \right] = ğ›½^2 $$

$$ ğœŒ_{ğ‘Ÿ_ğ¼, ğ‘Ÿ_{ğ‘˜ \gt ğ‘›}} = \frac{ğ›½^2}{\sqrt{ğ›½^2 + \frac{1âˆ’ğ›½^2}{ğ‘›}}} âŸ¹ ğ›½ = \sqrt{ \rho_{ğ‘Ÿ_ğ¼, ğ‘Ÿ_{ğ‘˜ \gt ğ‘›}} \sigma_I } = \rho_{ğ‘Ÿ_s, ğ‘Ÿ_{ğ‘˜ \gt ğ‘›}} $$

Then, analogously as before:

$$ \hat{\rho_{ğ‘Ÿ_s, ğ‘Ÿ_{ğ‘˜>ğ‘›}}} = \sqrt{ \hat{\rho_{ğ‘Ÿ_ğ¼, ğ‘Ÿ_{ğ‘˜ \gt ğ‘›}}} \hat{\sigma_I} } $$ 

It may seem counter-intuitive that we derive (adjusted) estimators of certain parameters using assumptions of the underlying distributions which determine these parameters. However, the goal here is to present the impact of endogeneity on the commonly used estimators and show that if these assumptions are satisfied, the proposed adjustments yield desirable results. Although such simplistic conditions cannot be assumed to hold in reality, they are very good for illustrative purposes, because they allow to present general tendencies in a straightforward way. This is done in section 'Simple framework' in the notebook [Endogeneity_in_the_CAPM](/Endogeneity_in_the_CAPM.ipynb). 

In the next section we will relax certain assumptions to allow the adjusted estimators to be applied in realistic conditions.


## **Coefficients in a complex framework**

Consider the following framework: 
- We have $ğ‘â‰¥2$ market factors in a cluster, $ğ‘›âˆˆ[2,ğ‘]$ of them compose an index.
- We assume that each index component market factor $ğ‘—=1,â€¦,ğ‘›$ has some assigned weight ($ğ‘¤_ğ‘—$), which is known <i>a priori</i>, and $\sum_{ğ‘—=1}^{ğ‘›} ğ‘¤_ğ‘— = 1$
- Furthermore, each market factor $ğ‘–=1,â€¦,ğ‘$ in a cluster has some assigned volatility ($ğœ_ğ‘–$) and beta ($ğ›½_ğ‘–$), which are unknown <i>a priori</i>.
- We assume that:

$$ \forall_{ğ‘—=1,â€¦,ğ‘›;ğ‘–=1,â€¦,ğ‘} {ğ‘¤_ğ‘—, ğœ_ğ‘–, ğ›½_ğ‘– \gt 0} $$

$$ \forall_{ğ‘—=1,â€¦,ğ‘›} {ğ‘¤_ğ‘— ğ›½_ğ‘— â‰¤ \frac{1}{2} \sum_{ğ‘™=1}^{ğ‘›} ğ‘¤_ğ‘™ ğ›½_ğ‘™} $$

- Additionally, we assume the systematic component return follows a standard normal distribution, and all market factorsâ€™ returns follow a normal distribution with expected value 0 and variance $ğœ_ğ‘–^2$, that is:

$$ ğ‘Ÿ_ğ‘  \sim ğ‘(0,1) $$

$$ \forall_{ğ‘–=1,â€¦,ğ‘} {ğ‘Ÿ_ğ‘– \sim ğ‘ \left( 0, ğœ_ğ‘–^2 \right)} $$

We want to calibrate coefficients of correlation with the systematic component for all market factors in a cluster over some time interval $ğ‘‡$.

Correlation with the systematic component:

$$ \forall_{ğ‘–=1,â€¦,ğ‘} {ğ›½_ğ‘– = ğœŒ_{ğ‘Ÿ_ğ‘ ,ğ‘Ÿ_ğ‘–} ğœ_ğ‘–; ğœŒ_{ğ‘Ÿ_ğ‘ ,ğ‘Ÿ_ğ‘–} = \frac{ğ›½_ğ‘–}{ğœ_ğ‘–}} $$

Variance of the idiosyncratic component:

$$ \forall_{ğ‘–=1,â€¦,ğ‘} ğ‘£ğ‘ğ‘Ÿ \left( ğ‘Ÿ_ğ‘– \right) = ğ‘£ğ‘ğ‘Ÿ \left( ğ›½_ğ‘– ğ‘Ÿ_ğ‘  + ğœ€_ğ‘– \right) = ğœ_{ğ‘–}^{2} âŸ¹ ğ‘£ğ‘ğ‘Ÿ \left( ğœ€_ğ‘– \right) = ğœ_{ğ‘–}^{2} âˆ’ ğœŒ_{ğ‘Ÿ_ğ‘ ,ğ‘Ÿ_ğ‘–}^{2} ğœ_{ğ‘–}^{2} = ğœ_ğ‘–^2 \left( 1 âˆ’ ğœŒ_{ğ‘Ÿ_ğ‘ ,ğ‘Ÿ_ğ‘–}^{2} \right) $$

Index return and its variance:

$$ ğ‘Ÿ_ğ¼ = ğ‘¤_1 \left( ğ›½_1 ğ‘Ÿ_ğ‘  + ğœ€_1 \right) + ğ‘¤_2 \left( ğ›½_2 ğ‘Ÿ_ğ‘  + ğœ€_2 \right) + â€¦ + ğ‘¤_ğ‘› \left( ğ›½_ğ‘› ğ‘Ÿ_ğ‘  + ğœ€_ğ‘› \right) = \sum_{ğ‘—=1}^{ğ‘›} ğ‘¤_ğ‘— ğ›½_ğ‘— ğ‘Ÿ_ğ‘  + \sum_{ğ‘—=1}^{ğ‘›} ğ‘¤_ğ‘— ğœ€_ğ‘— $$

$$ ğœ_ğ¼^2 â‰¡ ğ‘£ğ‘ğ‘Ÿ(ğ‘Ÿ_ğ¼) = ğ‘£ğ‘ğ‘Ÿ \left( \sum_{ğ‘—=1}^{ğ‘›} ğ‘¤_ğ‘— ğ›½_ğ‘— ğ‘Ÿ_ğ‘  + \sum_{ğ‘—=1}^{ğ‘›} ğ‘¤_ğ‘— ğœ€_ğ‘— \right) = ğ¸ \left[ \left( \sum_{ğ‘—=1}^{ğ‘›} ğ‘¤_ğ‘— ğ›½_ğ‘— ğ‘Ÿ_ğ‘  \right)^2 \right] + \sum_{ğ‘—=1}^{ğ‘›} w_ğ‘—^2 ğ¸ \left[ ğœ€_ğ‘—^2 \right] = \left( \sum_{ğ‘—=1}^{ğ‘›} ğ‘¤_ğ‘— ğ›½_ğ‘— \right)^2 ğ¸ \left[ğ‘Ÿ_ğ‘ ^2 \right] + \sum_{ğ‘—=1}^{ğ‘›} ğ‘¤_ğ‘—^2 ğœ_ğ‘—^2 \left( 1 âˆ’ ğœŒ_{ğ‘Ÿ_ğ‘ ,ğ‘Ÿ_ğ‘—}^{2} \right) = \left( \sum_{ğ‘—=1}^{ğ‘›} ğ‘¤_ğ‘— ğ›½_ğ‘— \right)^2 + \sum_{ğ‘—=1}^{ğ‘›} ğ‘¤_ğ‘—^2 ğœ_ğ‘—^2 âˆ’ \sum_{ğ‘—=1}^{ğ‘›} ğ‘¤_ğ‘—^2 ğ›½_ğ‘—^2 $$

Covariance of a component market factor return:

$$ ğ‘ğ‘œğ‘£ \left( ğ‘Ÿ_ğ¼, ğ‘Ÿ_{ğ‘˜â‰¤ğ‘›} \right) = ğ¸ \left[ \left( \sum_{ğ‘—=1}^{ğ‘›} ğ‘¤_ğ‘— ğ›½_ğ‘— ğ‘Ÿ_ğ‘  + \sum_{ğ‘—=1}^{ğ‘›} ğ‘¤_ğ‘— ğœ€_ğ‘— \right) \left( ğ›½_{ğ‘˜â‰¤ğ‘›} ğ‘Ÿ_ğ‘  + ğœ€_{ğ‘˜â‰¤ğ‘›} \right) \right] = ğ¸ \left[ ğ›½_{ğ‘˜â‰¤ğ‘›} ğ‘Ÿ_ğ‘  \sum_{ğ‘—=1}^{ğ‘›} ğ‘¤_ğ‘— ğ›½_ğ‘— ğ‘Ÿ_ğ‘  + ğ‘¤_{ğ‘˜â‰¤ğ‘›} ğœ€_{ğ‘˜â‰¤ğ‘›}^{2} \right] = \left( ğ›½_{ğ‘˜â‰¤ğ‘›} \sum_{ğ‘—=1}^{ğ‘›} ğ‘¤_ğ‘— ğ›½_ğ‘— \right) ğ¸ \left[ ğ‘Ÿ_ğ‘ ^2 \right] + ğ‘¤_{ğ‘˜â‰¤ğ‘›} ğ¸ \left[ ğœ€_{ğ‘˜â‰¤ğ‘›}^{2} \right] = ğ›½_{ğ‘˜â‰¤ğ‘›} \sum_{ğ‘—=1}^{ğ‘›} ğ‘¤_ğ‘— ğ›½_ğ‘— + ğ‘¤_{ğ‘˜â‰¤ğ‘›} ğœ_{ğ‘˜â‰¤ğ‘›}^{2} âˆ’ ğ‘¤_{ğ‘˜â‰¤ğ‘›} ğ›½_{ğ‘˜â‰¤ğ‘›}^{2} $$

Covariance of a non-component market factor return:

$$ ğ‘ğ‘œğ‘£ \left( ğ‘Ÿ_ğ¼, ğ‘Ÿ_{ğ‘˜>ğ‘›} \right) = ğ¸ \left[ \left( \sum_{ğ‘—=1}^{ğ‘›} ğ‘¤_ğ‘— ğ›½_ğ‘— ğ‘Ÿ_ğ‘  + \sum_{ğ‘—=1}^{ğ‘›} ğ‘¤_ğ‘— ğœ€_ğ‘— \right) \left( ğ›½_{ğ‘˜>ğ‘›} ğ‘Ÿ_ğ‘  + ğœ€_{ğ‘˜>ğ‘›} \right) \right] = ğ¸ \left[ ğ›½_{ğ‘˜>ğ‘›} ğ‘Ÿ_ğ‘  \sum_{ğ‘—=1}^{ğ‘›} ğ‘¤_ğ‘— ğ›½_ğ‘— ğ‘Ÿ_ğ‘  \right] =\left( ğ›½_{ğ‘˜>ğ‘›} \sum_{ğ‘—=1}^{ğ‘›} ğ‘¤_ğ‘— ğ›½_ğ‘— \right) ğ¸ \left[ ğ‘Ÿ_ğ‘ ^2 \right] = ğ›½_{ğ‘˜>ğ‘›} \sum_{ğ‘—=1}^{ğ‘›} ğ‘¤_ğ‘— ğ›½_ğ‘— $$


## **Proposition of coefficient adjustment**

Denote: 

$$ \overline{ğ›½} \equiv \sum_{ğ‘—=1}^{ğ‘›} ğ‘¤_ğ‘— ğ›½_ğ‘— $$ 

If we can obtain $\overline{ğ›½}$, we will get:

$$ ğ‘¤_{ğ‘˜â‰¤ğ‘›} ğ›½_{ğ‘˜â‰¤ğ‘›}^{2} âˆ’ ğ›½_{ğ‘˜â‰¤ğ‘›} \overline{ğ›½} + ğ‘ğ‘œğ‘£ \left( ğ‘Ÿ_ğ¼, ğ‘Ÿ_{ğ‘˜â‰¤ğ‘›} \right) âˆ’ ğ‘¤_{ğ‘˜â‰¤ğ‘›} ğœ_{ğ‘˜â‰¤ğ‘›}^{2} = 0 $$

$$ ğ‘ğ‘œğ‘£ \left( ğ‘Ÿ_ğ¼, ğ‘Ÿ_{ğ‘˜>ğ‘›} \right) = ğ›½_{ğ‘˜>ğ‘›} \overline{ğ›½} âŸ¹ ğ›½_{ğ‘˜>ğ‘›} = \frac{ ğ‘ğ‘œğ‘£ \left( ğ‘Ÿ_ğ¼, ğ‘Ÿ_{ğ‘˜>ğ‘›} \right) }{ \overline{ğ›½} } $$

We will leverage on the below formula:

$$ ğœ_ğ¼^2 = \left( \sum_{ğ‘—=1}^{ğ‘›} ğ‘¤_ğ‘— ğ›½_ğ‘— \right)^2 + \sum_{ğ‘—=1}^{ğ‘›} ğ‘¤_ğ‘—^2 ğœ_ğ‘—^2 âˆ’ \sum_{ğ‘—=1}^{ğ‘›} ğ‘¤_ğ‘—^2 ğ›½_ğ‘—^2 $$

Note that:

$$ \frac{ \sum_{ğ‘—=1}^{ğ‘›} ğ‘¤_ğ‘—^2 ğ›½_ğ‘—^2 }{ \left( \sum_{ğ‘—=1}^{ğ‘›} ğ‘¤_ğ‘— ğ›½_ğ‘— \right)^2 } = \frac{ \sum_{ğ‘˜=1,ğ‘™=1}^{ğ‘›} ğŸ™_{ğ‘˜=ğ‘™} ğ‘¤_ğ‘˜ ğ‘¤_ğ‘™ ğ›½_ğ‘˜ ğ›½_ğ‘™ }{ \sum_{ğ‘˜=1,ğ‘™=1}^{ğ‘›} ğ‘¤_ğ‘˜ ğ‘¤_ğ‘™ ğ›½_ğ‘˜ ğ›½_ğ‘™ } â‰ˆ \frac{ \sum_{ğ‘˜=1,ğ‘™=1}^{ğ‘›} ğŸ™_{ğ‘˜=ğ‘™} ğ‘¤_ğ‘˜ ğ‘¤_ğ‘™ }{ \sum_{ğ‘˜=1,ğ‘™=1}^{ğ‘›} ğ‘¤_ğ‘˜ ğ‘¤_ğ‘™ } = \sum_{ğ‘—=1}^{ğ‘›} ğ‘¤_ğ‘—^2 âŸ¹ ğœ_ğ¼^2 â‰ˆ \overline{ğ›½}^2 + \sum_{ğ‘—=1}^{ğ‘›} ğ‘¤_ğ‘—^2 ğœ_ğ‘—^2 âˆ’ \sum_{ğ‘—=1}^{ğ‘›} ğ‘¤_ğ‘—^2 \overline{ğ›½}^2 âŸ¹ \overline{ğ›½} â‰ˆ \sqrt{ \frac{ ğœ_ğ¼^2 âˆ’ \sum_{ğ‘—=1}^{ğ‘›} ğ‘¤_ğ‘—^2 ğœ_ğ‘—^2 }{ 1 âˆ’ \sum_{ğ‘—=1}^{ğ‘›} ğ‘¤_ğ‘—^2 } } $$

We solve for $ğ›½_{ğ‘˜â‰¤ğ‘›}$:

$$ ğ›½_{ğ‘˜â‰¤ğ‘›} = \frac{ \overline{ğ›½} \pm \sqrt{ \overline{ğ›½}^2 - 4 ğ‘¤_{ğ‘˜â‰¤ğ‘›} \left( ğ‘ğ‘œğ‘£ \left( ğ‘Ÿ_ğ¼, ğ‘Ÿ_{ğ‘˜â‰¤ğ‘›} \right) âˆ’ ğ‘¤_{ğ‘˜â‰¤ğ‘›} ğœ_{ğ‘˜â‰¤ğ‘›}^{2} \right) } }{ 2 ğ‘¤_{ğ‘˜â‰¤ğ‘›} } $$

We need to figure out which of the two solutions is the right one. When we substitute:

$$ ğ‘ğ‘œğ‘£ \left( ğ‘Ÿ_ğ¼, ğ‘Ÿ_{ğ‘˜â‰¤ğ‘›} \right) = ğ›½_{ğ‘˜â‰¤ğ‘›} \overline{ğ›½} âˆ’ ğ‘¤_{ğ‘˜â‰¤ğ‘›} ğ›½_{ğ‘˜â‰¤ğ‘›}^{2} + ğ‘¤_{ğ‘˜â‰¤ğ‘›} ğœ_{ğ‘˜â‰¤ğ‘›}^{2}, $$ 

we get:

$$ ğ›½_{ğ‘˜â‰¤ğ‘›} = \frac{ \overline{ğ›½} \pm \sqrt{ \overline{ğ›½}^2 - 4 ğ‘¤_{ğ‘˜â‰¤ğ‘›} \left( ğ›½_{ğ‘˜â‰¤ğ‘›} \overline{ğ›½} âˆ’ ğ‘¤_{ğ‘˜â‰¤ğ‘›} \beta_{ğ‘˜â‰¤ğ‘›}^{2} \right) } }{ 2 ğ‘¤_{ğ‘˜â‰¤ğ‘›} } = \frac{ \overline{ğ›½} }{ 2 ğ‘¤_{ğ‘˜â‰¤ğ‘›} } \pm \sqrt{ \left( \frac{ \overline{ğ›½} }{ 2 ğ‘¤_{ğ‘˜â‰¤ğ‘›} } - ğ›½_{ğ‘˜â‰¤ğ‘›} \right)^2 } = \begin{cases} \frac{\overline{ğ›½}}{ğ‘¤_{ğ‘˜â‰¤ğ‘›}} - ğ›½_{ğ‘˜â‰¤ğ‘›} \\ 
ğ›½_{ğ‘˜â‰¤ğ‘›} \end{cases} $$

This indicates that the second solution (with subtraction in the numerator) is the right one. Thus, we obtain the following estimators:

$$ \hat{\overline{\beta}} = \sqrt{ \frac{ \hat{ğœ_ğ¼^2} - \sum_{ğ‘—=1}^{ğ‘›} ğ‘¤_ğ‘—^2 \hat{ğœ_ğ‘—^2} }{ 1 âˆ’ \sum_{ğ‘—=1}^{ğ‘›} ğ‘¤_ğ‘—^2 } } $$

$$ \hat{ğ›½_{ğ‘˜>ğ‘›}} = \frac{ \hat{ğ‘ğ‘œğ‘£ \left( ğ‘Ÿ_ğ¼, ğ‘Ÿ_{ğ‘˜>ğ‘›} \right)} }{ \hat{\overline{\beta}} }; \hat{ ğœŒ_{ğ‘Ÿ_s,ğ‘Ÿ_{ğ‘˜>ğ‘›}} } = \frac{\hat{ğ›½_{ğ‘˜>ğ‘›}}}{\hat{ğœ_{ğ‘˜>ğ‘›}}} $$

$$ \hat{ğ›½_{ğ‘˜â‰¤ğ‘›}} = \frac{ \hat{\overline{ğ›½}} - \sqrt{ \hat{\overline{ğ›½}}^2 - 4 ğ‘¤_{ğ‘˜â‰¤ğ‘›} \left( \hat{ğ‘ğ‘œğ‘£ \left( ğ‘Ÿ_ğ¼, ğ‘Ÿ_{ğ‘˜â‰¤ğ‘›} \right)} âˆ’ ğ‘¤_{ğ‘˜â‰¤ğ‘›} \hat{ğœ_{ğ‘˜â‰¤ğ‘›}^{2}} \right) } }{ 2 ğ‘¤_{ğ‘˜â‰¤ğ‘›} }; \hat{ ğœŒ_{ğ‘Ÿ_s,ğ‘Ÿ_{ğ‘˜â‰¤ğ‘›}} } = \frac{\hat{ğ›½_{ğ‘˜â‰¤ğ‘›}}}{\hat{ğœ_{ğ‘˜â‰¤ğ‘›}}} $$



